# baseURI: http://biohackathon.org/resource/vg

@prefix : <http://biohackathon.org/resource/vg#> .
@prefix owl: <http://www.w3.org/2002/07/owl#> .
@prefix rdf: <http://www.w3.org/1999/02/22-rdf-syntax-ns#> .
@prefix rdfs: <http://www.w3.org/2000/01/rdf-schema#> .
@prefix spin: <http://spinrdf.org/spin#> .
@prefix xsd: <http://www.w3.org/2001/XMLSchema#> .
@prefix edam: <http://edamontology.org/> .
@prefix faldo: <http://biohackathon.org/resource/faldo#> .

<http://biohackathon.org/resource/vg>
  rdf:type owl:Ontology ;
  <http://purl.org/dc/terms/license> <http://creativecommons.org/publicdomain/zero/1.0/> ;
  spin:imports <http://topbraid.org/spin/owlrl-all> ;
  spin:imports <http://topbraid.org/spin/rdfsplus> ;
  spin:imports <http://topbraid.org/spin/spinowl> ;
  owl:versionInfo "Created at the DBCLS RDF Summit 2, Sendai Japan and COVID-19 Virtual Biohackathon"^^xsd:string ;
.
:Node
  rdf:type owl:Class ;
  rdfs:comment "A node in the variant graph, representing a sequence section."^^xsd:string ;
  rdfs:label "Node"^^xsd:string ;
  rdfs:subClassOf owl:Thing ;
.
:Path
  rdf:type owl:Class ;
  rdfs:comment "A Path is a collection of steps from path to path that represent an asserdfs:labelmbled sequence integrated into the variant graph."^^xsd:string ;
  rdfs:label "Path"^^xsd:string ;
  rdfs:subClassOf owl:Thing ;
.
:Step
  rdf:type owl:Class ;
  rdfs:comment "A step along a path in the variant graph. A series of steps along a path represent an assembled sequence that was originally inserted into the variant graph. A step points to a :Node or the reverse complement of a node and has a rank (step number)."^^xsd:string ;
  rdfs:label "Step"^^xsd:string ;
  rdfs:subClassOf owl:Thing ;
.
:links
  rdf:type owl:ObjectProperty ;
  rdfs:comment "The super property that says two nodes are linked and does not allow one to infer which side to side it goes"^^xsd:string ;
  rdfs:domain :Node ;
  rdfs:label "links"^^xsd:string ;
  rdfs:range :Node ;
.
:linksForwardToForward
  rdf:type owl:ObjectProperty ;
  rdfs:subPropertyOf :links ;
  rdfs:comment "This links a node from the forward (5' to 3') strand on the subject node to the forward (5' to 3') strand on the predicate node."^^xsd:string ;
  rdfs:domain :Node ;
  rdfs:label "++"^^xsd:string ;
  rdfs:label "linksForwardToForward"^^xsd:string ;
  rdfs:range :Node ;
.
:linksForwardToReverse
  rdf:type owl:ObjectProperty ;
  rdfs:subPropertyOf :links ;
  rdfs:comment "This links a node from the forward (5' to 3') strand on the subject node to the reverse (3' to 5') strand on the predicate node."^^xsd:string ;
  rdfs:domain :Node ;
  rdfs:label "+-"^^xsd:string ;
  rdfs:label "linksForwardToReverse"^^xsd:string ;
  rdfs:range :Node ;
.
:linksReverseToForward
  rdf:type owl:ObjectProperty ;
  rdfs:subPropertyOf :links ;
  rdfs:comment "This links a node from the reverse (3' to 5') strand on the subject node to the forward (5' to 3') strand on the predicate node."^^xsd:string ;
  rdfs:domain :Node ;
  rdfs:label "-+"^^xsd:string ;
  rdfs:label "linksReverseToForward"^^xsd:string ;
  rdfs:range :Node ;
.
:linksReverseToReverse
  rdf:type owl:ObjectProperty ;
  rdfs:subPropertyOf :links ;
  rdfs:comment "This links a node from the reverse (3' to 5') strand on the subject node to the reverse (3' to 5') strand on the predicate node."^^xsd:string ;
  rdfs:domain :Node ;
  rdfs:label "--"^^xsd:string ;
  rdfs:label "linksReverseToReverse"^^xsd:string ;
  rdfs:range :Node ;
.
:node
  rdf:type owl:ObjectProperty ;
  rdfs:comment "This means that this step occurs on the forward strand of the sequence attaced to the node (i.e. it is on the explicit encoded forward (5' to 3') strand) of the predicate node."^^xsd:string ;
  rdfs:domain :Step ;
  rdfs:label "node"^^xsd:string ;
  rdfs:range :Node ;
.
:path
  rdf:type owl:ObjectProperty ;
  rdfs:comment "This means that this step occurs on the path that is the object of this statment"^^xsd:string ;
  rdfs:domain :Step ;
  rdfs:label "path"^^xsd:string ;
  rdfs:range :Path ;
.

:position
  rdf:type owl:ObjectProperty ;
  rdfs:comment "This is the position on the reference path at which this step starts."^^xsd:string ;
  rdfs:domain :Step ;
  rdfs:label "position"^^xsd:string ;
  rdfs:range xsd:positiveInteger .

:rank
  rdf:type owl:DatatypeProperty ;
  rdfs:comment "The rank records the step place along its path."^^xsd:string ;
  rdfs:domain :Step ;
  rdfs:label "rank"^^xsd:string ;
  rdfs:range xsd:positiveInteger ;
.
:reverseOfNode
  rdf:type owl:ObjectProperty ;
  rdfs:comment "This means this step occurs on the revese complement of the sequence attaced to the node (i.e. it is on the implicit reverse (3' to 5') strand) of the predicate node."^^xsd:string ;
  rdfs:domain :Step ;
  rdfs:label "reverseOfNode"^^xsd:string ;
  rdfs:range :Node ;
.
:ZoomLevel
  rdf:type owl:Class ;
  rdfs:comment "A zoom level of Pangenome."^^xsd:string ;
  rdfs:label "ZoomLevel"^^xsd:string ;
  rdfs:subClassOf owl:Thing ;
.
:zoomFactor
  rdf:type owl:DatatypeProperty ;
  rdfs:comment "The zoom factor of pangenome, which is defined as bin width, generally."^^xsd:string ;
  rdfs:domain :ZoomLevel ;
  rdfs:label "zoomFactor"^^xsd:string ;
  rdfs:range xsd:positiveInteger ;
.
:components
  rdf:type owl:ObjectProperty ;
  rdfs:comment "A zoom level has one or more components."^^xsd:string ;
  rdfs:domain :ZoomLevel ;
  rdfs:label "components"^^xsd:string ;
  rdfs:range :Component ;
.
:Component
  rdf:type owl:Class ;
  rdfs:comment "A region between Links structuring all bins and their present individuals into one component."^^xsd:string ;
  rdfs:label "Component"^^xsd:string ;
  rdfs:subClassOf owl:Thing ;
.
:forwardComponentEdge
  rdf:type owl:ObjectProperty ;
  rdfs:comment "The super property that says two components are linked in forward orientation on the pangenome sequence."^^xsd:string ;
  rdfs:domain :Component ;
  rdfs:label "forwardComponentEdge"^^xsd:string ;
  rdfs:range :Component ;
.
:reverseComponentEdge
  rdf:type owl:ObjectProperty ;
  owl:inverseOf :forwardComponentEdge ;
  rdfs:comment "The super property that says two components are linked in reverse orientation on the pangenome sequence."^^xsd:string ;
  rdfs:domain :Component ;
  rdfs:label "reverseComponentEdge"^^xsd:string ;
  rdfs:domain :Component ;
.
:componentRank
  rdf:type owl:DatatypeProperty ;
  rdfs:comment "The rank records that step place along its pangenome sequence."^^xsd:string ;
  rdfs:domain :Component ;
  rdfs:label "componentRank"^^xsd:string ;
  rdfs:range xsd:positiveInteger ;
.
:bins
  rdf:type owl:ObjectProperty ;
  rdfs:comment "A Component has one or more Bins."^^xsd:string ;
  rdfs:domain :Component ;
  rdfs:label "bins"^^xsd:string ;
  rdfs:range :Bin ;
.
:Bin
  rdf:type owl:Class ;
  rdfs:comment "A bin in the output of odgi bin, representing a sequence section."^^xsd:string ;
  rdfs:label "Bin"^^xsd:string ;
  rdfs:subClassOf owl:Thing ;
.
:binRank
  rdf:type owl:DatatypeProperty ;
  rdfs:comment "The rank records that step place along its pangenome sequence."^^xsd:string ;
  rdfs:domain :Bin ;
  rdfs:label "binRank"^^xsd:string ;
  rdfs:range xsd:positiveInteger ;
.
:forwardBinEdge
  rdf:type owl:ObjectProperty ;
  owl:inverseOf :reverseBinEdge ;
  rdfs:comment "The super property that says two bins are linked in forward orientation on the pangenome sequence."^^xsd:string ;
  rdfs:domain :Bin ;
  rdfs:label "forwardBinEdge"^^xsd:string ;
  rdfs:domain :Bin ;
.
:reverseBinEdge
  rdf:type owl:ObjectProperty ;
  owl:inverseOf :forwardBinEdge ;
  rdfs:comment "The super property that says two bins are linked in reverse orientation on the pangenome sequence."^^xsd:string ;
  rdfs:domain :Bin ;
  rdfs:label "reverseBinEdge"^^xsd:string ;
  rdfs:domain :Bin ;
.
:Link
  rdf:type owl:Class ;
  rdfs:comment "A link marks a graph traversal along a nonlinear connection."^^xsd:string ;
  rdfs:label "Link"^^xsd:string ;
  rdfs:subClassOf owl:Thing ;
.
:arrival
  rdf:type owl:ObjectProperty ;
  rdfs:comment "An end bin of nonlinear link. Incoming edge of the bin."^^xsd:string ;
  owl:inverseOf :departure;
  rdfs:domain :Link ;
  rdfs:label "arrival"^^xsd:string ;
  rdfs:range :Bin ;
.
:departure
  rdf:type owl:ObjectProperty ;
  rdfs:comment "A start bin of nonlinear link. Outgoing edge of the bin."^^xsd:string ;
  owl:inverseOf :arrival;
  rdfs:domain :Link ;
  rdfs:label "departure"^^xsd:string ;
  rdfs:range :Bin ;
.
:linkPaths
  rdf:type owl:ObjectProperty ;
  rdfs:comment "A list of paths that follow the same non-linear link between two bins."^^xsd:string ;
  rdfs:domain :Link ;
  rdfs:label "linkPaths"^^xsd:string ;
  rdfs:range :Path ;
.
:forwardLinkEdge
  rdf:type owl:ObjectProperty ;
  rdfs:comment "The super property that says two links are linked in forward orientation on the link column."^^xsd:string ;
  rdfs:domain :Link ;
  rdfs:label "forwardLinkEdge"^^xsd:string ;
  rdfs:range :Link ;
.
:reverseLinkEdge
  rdf:type owl:ObjectProperty ;
  owl:inverseOf :forwardLinkEdge ;
  rdfs:comment "The super property that says two links are linked in reverse orientation on the link column."^^xsd:string ;
  rdfs:domain :Link ;
  rdfs:label "reverseLinkEdge"^^xsd:string ;
  rdfs:domain :Link ;
.
:linkRank
  rdf:type owl:DatatypeProperty ;
  rdfs:comment "The rank records that step place along a link column."^^xsd:string ;
  rdfs:domain :Link ;
  rdfs:label "linkRank"^^xsd:string ;
  rdfs:range xsd:positiveInteger ;
.
:linkZoomLevel
  rdf:type owl:ObjectProperty ;
  rdfs:comment "A link is related to each zoom level."^^xsd:string ;
  rdfs:domain :Link ;
  rdfs:label "linkZoomLevel"^^xsd:string ;
  rdfs:range :ZoomLevel ;
.
:cells
  rdf:type owl:ObjectProperty ;
  rdfs:comment "A Bin has one or more paths of a specific group (component) of a specific zoom. That is represented as cells on the matrix."^^xsd:string ;
  rdfs:domain :Bin ;
  rdfs:label "cells"^^xsd:string ;
  rdfs:range :Cell ;
.
:Cell
  rdf:type owl:Class ;
  rdfs:comment "A cell along a path of a specific group (component) of a specific zoom. A cell to a :Component and a :Path with supplemental informations."^^xsd:string ;
  rdfs:label "Cell"^^xsd:string ;
  rdfs:subClassOf owl:Thing ;
.
:cellRegions
  rdf:type owl:ObjectProperty ;
  rdfs:comment "A cell is composed of the specific subsequence of paths."^^xsd:string ;
  rdfs:domain :Cell ;
  rdfs:label "cellRegions"^^xsd:string ;
  rdfs:range faldo:Region ;
.
:positionPercent
  rdf:type owl:DatatypeProperty ;
  rdfs:comment "The position coverage percent of the path in the component."^^xsd:string ;
  rdfs:domain :Cell ;
  rdfs:label "positionPercent"^^xsd:string ;
  rdfs:range xsd:float ;
.
:inversionPercent
  rdf:type owl:DatatypeProperty ;
  rdfs:comment "The inversion percent of the path in the component."^^xsd:string ;
  rdfs:domain :Cell ;
  rdfs:label "inversionPercent"^^xsd:string ;
  rdfs:range xsd:float ;
.
:VG_Format
  a owl:Class ;
  rdfs:subClassOf edam:format_2921, edam:format_2055 ;
  rdfs:label "Graph" ;
  rdfs:comment "Consists of nodes, edges, and paths. Nodes each have a unique ID and a DNA sequence, edges consist of two node sides (so the graph is bidirected), and paths are a sequence of nodes and orientations. Paths also have names." ;
  rdfs:isDefinedBy <https://raw.githubusercontent.com/vgteam/libvgio/master/deps/vg.proto> ;
.
:GAM_Format
  a owl:Class ;
  rdfs:label "Alignment" ;
  rdfs:subClassOf edam:format_2055 ;
  rdfs:comment "Contains an alignment to a graph" ;
  rdfs:isDefinedBy <https://raw.githubusercontent.com/vgteam/libvgio/master/deps/vg.proto> ;
.
:GAMP_Format
  a owl:Class ;
  rdfs:label "MultipathAlignment" ;
  rdfs:comment "Contains a DAG of subalignments to different paths through the reference graph" ;
  rdfs:isDefinedBy <https://raw.githubusercontent.com/vgteam/libvgio/master/deps/vg.proto> ;
.
:Snarl_Format
  a owl:Class ;
  rdfs:label "Snarl" ;
  rdfs:comment " A series of Snarl objects, each of which contain: The boundaries of a snarl (a bubble-like motif in a graph), the snarl (if any) that contains this one, classifications of the snarl based on the reachability of the two boundary nodes from each other and the cyclic-ness of the subcomponent." ;
  rdfs:isDefinedBy <https://raw.githubusercontent.com/vgteam/libvgio/master/deps/vg.proto> ;
.
:Snarl_Traversal_Format
  a owl:Class ;
  rdfs:label "SnarlTraversal" ;
  rdfs:comment " A series of SnarlTraversal objects, each of which contain: A walk in the graph through a Snarl, and optionally a name." ;
  rdfs:isDefinedBy <https://raw.githubusercontent.com/vgteam/libvgio/master/deps/vg.proto> ;
.
:XG_Format
  a owl:Class ;
  rdfs:label "XG" ;
  rdfs:comment "An immutable, succinct representation of a graph. Contains the same info as the .vg." ;
  rdfs:seeAlso :VG_Format ;
  rdfs:isDefinedBy <https://raw.githubusercontent.com/vgteam/libvgio/master/deps/vg.proto> ;
.
:GCSA2_Format
  a owl:Class ;
  rdfs:label "GCSA2" ;
  rdfs:comment "Generalized compressed suffix array 2, an exact match index published by Jouni Siren" ;
  rdfs:isDefinedBy <https://raw.githubusercontent.com/vgteam/libvgio/master/deps/vg.proto> ;
.
:GBWT_Format 
  a owl:Class ;
  rdfs:label "GBWT" ;
  rdfs:comment "Graph Burrows-Wheeler Transform, a succinct collection of paths through a genome graph, published by Jouni Siren. Usually represents haplotypes." ;
  rdfs:isDefinedBy <https://raw.githubusercontent.com/vgteam/libvgio/master/deps/vg.proto> ;
.
